src/HOL/Corec_Examples/Stream_Processor.thy
@@ -61,26 +61,20 @@ by(subst run.code; simp; fail)+
 lemma copy_sel[simp]: "out copy = Get (\<lambda>a. Put a copy)"
   by (subst copy.code; simp)
 
-lemma wf_imp_irrefl:
-  assumes "wf r" shows "irrefl r" 
-  using wf_irrefl [OF assms] by (auto simp add: irrefl_def)
-
-
 corecursive sp_comp (infixl "oo" 65) where
   "sp oo sp' = (case (out sp, out sp') of
       (Put b sp, _) \<Rightarrow> In (Put b (sp oo sp'))
     | (Get f, Put b sp) \<Rightarrow> In (f b) oo sp
     | (_, Get g) \<Rightarrow> get (\<lambda>a. (sp oo In (g a))))"
-  apply(relation "map_prod In In ` sub <*lex*> map_prod In In ` sub")
-    apply(auto simp: inj_on_def out_def split: sp\<^sub>\<nu>.splits intro: wf_map_prod_image)
-  by (metis Get_neq)
+  by (relation "map_prod In In ` sub <*lex*> map_prod In In ` sub")
+    (auto simp: inj_on_def out_def split: sp\<^sub>\<nu>.splits intro: wf_map_prod_image)
 
 lemma run_copy_unique:
-  "(\<And>s. h s = shd s ## h (stl s)) \<Longrightarrow> h = run copy"
-  apply corec_unique
-  apply(rule ext)
-  apply(subst copy.code)
-  apply simp
-  done
+    "(\<And>s. h s = shd s ## h (stl s)) \<Longrightarrow> h = run copy"
+apply corec_unique
+apply(rule ext)
+apply(subst copy.code)
+apply simp
+done
 
 end
